Fix the definition of horizontal composition
When one of the components interacts with the environment, the
environment may then want to resume the other module. This means that
we need to recombine the interaction's continuation with the suspended
continuation of the other component, similarly to how the entry
continuations are initially combined.

One consequence of this is that we need to assign a query domain not
just to the module as a whole, but to every continuation. The definition
of RTS behaviors is modified accordingly.

Taking all this into account, I restructure horizontal composition
into: 1. a flat composition operator that runs the two components side
by side and handles this combination of continuations to switch between
the components as needed; 2. a resolution operator which allows the
combined component to interact with itself, by making sure that queries
made to the environment are immediately diverted to the component's own
continuation whenever possible, so that the external interaction is
replaced with an internal action.

games/Composition.v
@@ -12,241 +12,214 @@ Require Import Classical.
 Require Import Axioms.
 
 
-(** * Horizontal composition *)
+(** * Flat composition *)
 
-Module HComp.
+Module FComp.
   Import RTS.
 
-  Section RTS.
-    Context {G A} (sw : output G -> option (input G)) (α : rts G A).
+  (** ** Definition *)
 
-    Inductive hc_state : Type :=
-      | hc_r (a : A) (k : input G -> A)
-      | hc_z.
+  (** Given a RTS, we can create a new RTS that maintains the states
+    of two threads within this RTS. At any time, only one of the
+    threads will be running and we will store a suspended continuation
+    for the inactive thread. *)
 
-    Definition hc_behavior (r : RTS.behavior G A) (k : input G -> A) :=
-      match r with
-        | internal a =>
-          internal (hc_r a k)
-        | interacts mo k' =>
-          match sw mo with
-            | Some m => internal (hc_r (k m) k')
-            | None => interacts mo (fun mi => hc_r (k' mi) k)
-          end
-        | diverges =>
-          diverges
-        | goes_wrong =>
-          goes_wrong
-      end.
+  Inductive state {G A} :=
+    | running (a : A) (k : input G -> option A)
+    | conflict.
 
-    Inductive hc : rts G hc_state :=
-      | hc_intro a k r :
-          α a r ->
-          hc (hc_r a k) (hc_behavior r k).
+  Arguments state : clear implicits.
 
-  End RTS.
+  (** Two continuations for the underlying can be combined into a
+    continuation for the two-threaded RTS in the following way. *)
 
-  Arguments hc_state : clear implicits.
+  Definition liftk {G A} (k1 k2 : input G -> option A) (q : input G) :=
+    match k1 q, k2 q with
+      | None, None => None
+      | Some a1, None => Some (running a1 k2)
+      | None, Some a2 => Some (running a2 k1)
+      | Some _, Some _ => Some conflict
+    end.
+
+  (** When the running thread interacts with the environment, its
+    continuation will be combined with the suspended continuation, so
+    that the environment may resume either thread. *)
+
+  Definition liftb {G A} (r : behavior G A) k :=
+    match r with
+      | internal a' => internal (running a' k)
+      | interacts mo k' => interacts mo (liftk k' k)
+      | diverges => diverges
+      | goes_wrong => goes_wrong
+    end.
+
+  Inductive step {G A} (α : rts G A) : rts G (state G A) :=
+    step_intro a k r :
+      α a r ->
+      step α (running a k) (liftb r k).
 
   (** ** Monotonicity *)
 
-  Inductive hc_rel {G A B} R : rel (hc_state G A) (hc_state G B) :=
-    | hc_r_rel :
-        Monotonic hc_r (R ++> (- ==> R) ++> hc_rel R)
-    | hc_z_rel :
-        Monotonic hc_z (hc_rel R).
+  Inductive state_rel {G A B} R : rel (state G A) (state G B) :=
+    | running_rel :
+        Monotonic running (R ++> (- ==> option_rel R) ++> state_rel R)
+    | conflict_rel :
+        Monotonic conflict (state_rel R).
 
-  Global Existing Instance hc_r_rel.
-  Global Existing Instance hc_z_rel.
-  Global Instance hc_r_rel_params : Params (@hc_r) 2.
+  Global Existing Instance running_rel.
+  Global Existing Instance conflict_rel.
+  Global Instance running_rel_params : Params (@running) 2.
 
-  Global Instance hc_behavior_rel {G A B} R sw :
+  Global Instance liftk_sim :
     Monotonic
-      (hc_behavior sw)
-      (behavior_le R ++> (- ==> R) ++> behavior_le (@hc_rel G A B R)).
+      (@liftk)
+      (forallr -, forallr R,
+        (- ==> option_rel R) ++>
+        (- ==> option_rel R) ++>
+        (- ==> option_rel (state_rel R))).
   Proof.
-    unfold hc_behavior. rauto.
+    unfold liftk. rauto.
   Qed.
 
-  Global Instance hc_behavior_rel_params :
-    Params (@hc_behavior) 2.
-
-  Global Instance hc_sim {G A B} R :
-    Monotonic hc (- ==> sim R ++> sim (@hc_rel G A B R)).
+  Global Instance liftb_sim :
+    Monotonic
+      (@liftb)
+      (forallr -, forallr R,
+        behavior_le R ++>
+        (- ==> option_rel R) ++>
+        behavior_le (state_rel R)).
   Proof.
-    intros sw α β Hαβ sa sb Hs ka Hka.
-    destruct Hka as [a ka ra].
+    unfold liftb. rauto.
+  Qed.
+
+  Global Instance step_sim {G A B} R :
+    Monotonic step (sim R ++> sim (@state_rel G A B R)).
+  Proof.
+    intros α β Hαβ sa sb Hs ra Hra.
+    destruct Hra as [a ka ra Hra].
     inversion Hs as [xa b Hab xka kb Hk | ]; clear Hs; subst.
     edestruct Hαβ as (rb & Hrb & Hr); eauto.
-    exists (hc_behavior sw rb kb). split; [ | rauto].
-    constructor; auto.
+    exists (liftb rb kb). split.
+    - constructor; auto.
+    - rauto.
   Qed.
 
-  Global Instance hc_sim_params :
-    Params (@hc) 2.
+  Global Instance step_sim_params :
+    Params (@step) 1.
 
-  (** ** Properties *)
+  (** ** Modules *)
 
-  Lemma hc_behavior_external {G A} sw (r : behavior G A) (k : input G -> A) :
-    behavior_external (hc_behavior sw r k) ->
-    behavior_external r.
+  (** When we wish to compute the flat composition of two modules, we
+    can use the sum of the underlying RTS and combine the two initial
+    continuations. *)
+
+  Definition of {li} (α β : modsem li) : modsem li :=
+    {|
+      modsem_lts := step (modsem_lts α + modsem_lts β);
+      modsem_entry :=
+        liftk
+          (fun q => option_map inl (modsem_entry α q))
+          (fun q => option_map inr (modsem_entry β q));
+    |}.
+
+  Global Instance of_ref :
+    Monotonic (@of) (forallr -, modref ++> modref ++> modref).
   Proof.
-    destruct r; inversion 1; constructor.
+    intros li α1 β1 Hαβ1 α2 β2 Hαβ2.
+    pose proof Hαβ1 as [R1 H1 He1].
+    pose proof Hαβ2 as [R2 H2 He2].
+    exists (state_rel (R1 + R2)); simpl.
+    - apply step_sim.
+      rauto.
+    - intro q.
+      apply liftk_sim; repeat rstep; auto.
   Qed.
+End FComp.
 
-  Lemma hc_reachable {G A} sw (α : rts G A) a a' k :
-    reachable α a a' ->
-    reachable (hc sw α) (hc_r a k) (hc_r a' k).
+
+(** * Resolution operator *)
+
+Module Res.
+  Import RTS.
+
+  (** ** Definition *)
+
+  Definition res_behavior {G A} sw (r : behavior G A) : behavior G A :=
+    match r with
+      | interacts mo k =>
+        match sw mo with
+          | Some mi =>
+            match k mi with
+              | Some a' => internal a'
+              | None => r
+            end
+          | None => r
+        end
+      | _ => r
+    end.
+
+  Inductive res {G A} sw (α : rts G A) : rts G A :=
+    res_intro a r :
+      α a r ->
+      res sw α a (res_behavior sw r).
+
+  (** ** Monotonicity *)
+
+  Global Instance res_sim :
+    Monotonic (@res) (forallr -, forallr R, - ==> sim R ++> sim R).
   Proof.
-    induction 1; eauto.
-    econstructor; eauto.
-    change (internal _) with (hc_behavior sw (internal a') k).
-    constructor; eauto.
+    intros G A B R sw α β Hαβ a b Hab ra Hra.
+    destruct Hra as [a' ra Hra].
+    edestruct Hαβ as (rb & Hrb & Hr); eauto.
+    exists (res_behavior sw rb). split.
+    - constructor; auto.
+    - unfold res_behavior. rauto.
   Qed.
 
   (** ** Modules *)
 
-  Section HCOMP.
-    Context {li} (α1 α2 : modsem (li -o li)).
+  Definition sw li (mo : output (li -o li)) : option (input (li -o li)) :=
+    match mo with
+      | inr x => Some (inl x)
+      | inl x => Some (inr x)
+    end.
 
-    Definition hcomp_dom (q : query (li -o li)) : bool :=
-      modsem_dom α1 q || modsem_dom α2 q.
+  Definition of {li} (α : modsem (li -o li)) : modsem (li -o li) :=
+    {|
+      modsem_lts := res (sw li) α;
+      modsem_entry := modsem_entry α;
+    |}.
 
-    Definition hcomp_sw (q : reply (li -o li)) : option (query (li -o li)) :=
-      match q with
-        | inl q => if hcomp_dom (inr q) then Some (inr q) else None
-        | inr r => Some (inl r) (* XXX need to know whether outermost reply *)
-      end.
-
-    Definition hcomp_entry (q : query (li -o li)) :=
-      match modsem_dom α1 q, modsem_dom α2 q with
-        | true, false =>
-            hc_r (G := li -o li)
-              (inl (modsem_entry α1 q))
-              (fun m => inr (modsem_entry α2 m))
-        | false, true =>
-            hc_r (G := li -o li)
-              (inr (modsem_entry α2 q))
-              (fun m => inl (modsem_entry α1 m))
-        | _, _ =>
-            hc_z
-      end.
-
-    Definition hcomp : modsem (li -o li) :=
-      {|
-        modsem_lts := hc (G := li -o li) hcomp_sw (α1 + α2)%rts;
-        modsem_dom := hcomp_dom;
-        modsem_entry := hcomp_entry;
-      |}.
-  End HCOMP.
-
-  Global Instance hcomp_dom_ref :
-    Monotonic (@hcomp_dom) (forallr -, modref ++> modref ++> - ==> eq).
+  Global Instance of_sim :
+    Monotonic (@of) (forallr -, modref ++> modref).
   Proof.
-    unfold hcomp_dom. repeat rstep. f_equal; rauto.
+    intros li α β [R Hαβ He].
+    esplit; simpl; eauto. rauto.
   Qed.
 
-  Global Instance hcomp_sw_ref :
-    Monotonic (@hcomp_sw) (forallr -, modref ++> modref ++> - ==> eq).
-  Proof.
-    unfold hcomp_sw. rauto.
-  Qed.
+  (** ** Commutation with [obs] *)
 
-  Global Instance hcomp_ref :
-    Monotonic (@hcomp) (forallr -, modref ++> modref ++> modref).
-  Proof.
-    intros li α1 β1 Hαβ1 α2 β2 Hαβ2.
-    pose proof Hαβ1 as [Hd1 R1 H1 He1].
-    pose proof Hαβ2 as [Hd2 R2 H2 He2].
-    exists (hc_rel (R1 + R2)); simpl.
-    - intros q. rauto.
-    - replace (hcomp_sw β1 β2) with (hcomp_sw α1 α2).
-      + eapply hc_sim. rauto.
-      + apply functional_extensionality. intros i. rauto.
-    - intros q. unfold hcomp_entry.
-      rewrite <- Hd1, <- Hd2.
-      repeat rstep; simpl; eauto.
-  Qed.
-
-  (** ** [hcomp] and [obs] *)
-
-  (** We prove that [hcomp] semi-commutes with [obs], in the sense
+  (** We prove that [res] semi-commutes with [obs], in the sense
     that applying [obs] after horizontal composition only should yield
     the same result as applying it both before and after horizontal
-    composition. *)
+    composition: in particular, for any step of [obs (res sw α)],
+    there is a corresponding step of [obs (res sw (obs α))]. This is
+    used as a lemma in proofs of syntactic composition. The proof is
+    non-trivial both in the diverging and terminating cases. *)
 
-  CoInductive forever_switching {G A} sw (α : rts G A) : hc_state G A -> Prop :=
-    | forever_switching_intro a a' ra k s' :
-        reachable α a a' ->
-        α a' ra ->
-        behavior_external ra ->
-        hc_behavior sw ra k = internal s' ->
-        forever_switching sw α s' ->
-        forever_switching sw α (hc_r a k).
+  (** *** Divergence *)
 
-  Lemma forever_switching_internal {G A} sw (α : rts G A) s s' :
-    hc sw α s (internal s') ->
-    forever_switching sw α s' ->
-    forever_switching sw α s.
-  Proof.
-    intros Hs' Hd.
-    inversion Hs' as [a0 k0 ra0 Hra0]; clear Hs'.
-    destruct ra0; inversion H0; clear H0.
-    - destruct Hd.
-      inversion H2; clear H2; subst.
-      eapply (forever_switching_intro sw α a0 a'0); eauto.
-    - destruct sw as [mx|] eqn:Hmx; inversion H2; clear H2; subst.
-      eapply (forever_switching_intro sw α a0 a0); eauto.
-      simpl. rewrite Hmx. reflexivity.
-  Qed.
+  (** First, if [res sw α] diverges, we need to distinguish two subcases.
+    On one hand, the divergence may result from an infinite number of
+    terminating segments which are stiched together by internal
+    switching, resulting in an infinite sequence of internal
+    actions. On the other hand, it may be that [α] itself diverges,
+    with [res] simply passing along these internal actions; even in
+    this case, this may be preceded by a finite number of internal
+    switches.
 
-  Inductive hc_settles {G A} sw (α : rts G A) : rts G (hc_state G A) :=
-    | hc_settles_external a a' ra k r :
-        α a' ra ->
-        reachable α a a' ->
-        hc_behavior sw ra k = r ->
-        behavior_external r ->
-        hc_settles sw α (hc_r a k) r
-    | hc_settles_diverges a k :
-        forever_internal α a ->
-        hc_settles sw α (hc_r a k) diverges
-    | hc_settles_switch a a' ra k s' r :
-        α a' ra ->
-        reachable α a a' ->
-        behavior_external ra ->
-        hc_behavior sw ra k = internal s' ->
-        hc_settles sw α s' r ->
-        hc_settles sw α (hc_r a k) r.
-
-  Hint Constructors hc_settles.
-
-  Lemma hc_settles_internal {G A} sw (α : rts G A) s s' r :
-    hc sw α s (internal s') ->
-    hc_settles sw α s' r ->
-    hc_settles sw α s r.
-  Proof.
-    intros Hs' Hr.
-    inversion Hs' as [a k ra Hra]; clear Hs'; subst.
-    destruct ra; inversion H0; clear H0.
-    - destruct Hr; inversion H1; clear H1; subst.
-      + eapply (hc_settles_external sw α a a'0); eauto.
-      + eapply (hc_settles_diverges sw α a); eauto.
-        econstructor; eauto.
-      + eapply (hc_settles_switch sw α a a'0); eauto.
-    - destruct sw as [mx|] eqn:Hmx; inversion H1; clear H1; subst.
-      eapply (hc_settles_switch sw α a a (interacts m k0)); eauto.
-      simpl. rewrite Hmx. reflexivity.
-  Qed.
-
-  Inductive obs_hc {G A} sw (α : rts G A) : rts G (hc_state G A) :=
-    | obs_hc_settles s r :
-        hc_settles sw α s r ->
-        obs_hc sw α s r
-    | obs_hc_forever_switching s :
-        forever_switching sw α s ->
-        obs_hc sw α s diverges.
-
-  (** *** Alternative formulations for coinductive properties *)
+    In order to simplify the case analysis we introduce the following
+    positive formulation of divergence. *)
 
   Lemma forever_internal_nbr {G A} (α : rts G A) a :
     nonbranching α ->
@@ -263,168 +236,185 @@ Module HComp.
       econstructor; eauto.
   Qed.
 
-  Lemma forever_switching_inv_internal {G A} sw (α : rts G A) s s' :
-    deterministic α ->
-    forever_switching sw α s ->
-    hc sw α s (internal s') ->
-    forever_switching sw α s'.
-  Proof.
-    intros Hα Hs Hs'.
-    inversion Hs'; clear Hs'; subst.
-    destruct r; simpl in H; try now inversion H.
-    - inversion Hs as [a1 a2 ra l s2 Ha2 Hra Hs2 Hs2d]; clear Hs; subst.
-      inversion H; clear H; subst.
-      eapply (reachable_inv_reachable α a a' a2) in Ha2; eauto.
-      econstructor; eauto.
-    - destruct sw eqn:Hm; inversion H; clear H; subst.
-      inversion Hs; clear Hs; subst.
-      assert (a' = a).
-      {
-        destruct H2; eauto.
-        eelim (nonbranching_internal_external α a (interacts m k0)); eauto.
-      }
-      subst.
-      assert (ra = interacts m k0).
-      {
-        eapply Hα; eauto.
-      }
-      subst.
-      simpl in H5.
-      rewrite Hm in H5.
-      inversion H5.
-      congruence.
-  Qed.
+  (** The formulation above is only valid when [α] is nonbranching,
+    otherwise [Σ n . τ^n] may be mistaken for [τ^ω]. To apply it to
+    [obs (res sw α)] we use the following lemmas. *)
 
-  Lemma forever_switching_nbr {G A} sw (α : rts G A) s :
+  Lemma res_det {G A} sw (α : rts G A) :
     deterministic α ->
-    forever_switching sw α s <->
-    (s <> hc_z /\
-     forall a k, reachable (hc sw α) s (hc_r a k) ->
-                 exists a' r s', reachable α a a' /\
-                                 α a' r /\
-                                 behavior_external r /\
-                                 hc_behavior sw r k = internal s').
-  Proof.
-    intros Hα. split.
-    - intros Hs.
-      split. { destruct Hs. congruence. }
-      intros a k Hak.
-      remember (hc_r a k) as s' eqn:Hs' in Hak.
-      revert a k Hs'.
-      induction Hak; intros.
-      + destruct Hs.
-        inversion Hs'; clear Hs'; subst.
-        exists a', ra, s'. eauto.
-      + eapply IHHak; eauto.
-        eapply forever_switching_inv_internal; eauto.
-    - revert s. cofix IH. intros s [Hnz Hs].
-      destruct s as [a k | ]; try congruence.
-      edestruct (Hs a k) as (a' & r & s' & Ha' & Hr & Hrext & Hs'); [ eauto .. | ].
-      eapply (forever_switching_intro sw α a a' r k); eauto.
-      eapply IH.
-      split. { destruct r; simpl in Hs'; try congruence.
-               destruct sw; congruence. }
-      intros.
-      eapply Hs.
-      transitivity s'; auto.
-      transitivity (hc_r a' k); auto using hc_reachable.
-      econstructor; eauto.
-      rewrite <- Hs'. constructor. auto.
-  Qed.
-
-  Lemma hc_det {G A} sw (α : rts G A) :
-    deterministic α ->
-    deterministic (hc sw α).
+    deterministic (res sw α).
   Proof.
     intros Hα s x y Hx Hy.
     destruct Hx. inversion Hy.
     f_equal; eauto.
   Qed.
 
-  Lemma forever_hc {G A} sw (α : rts G A) s :
-    deterministic α ->
-    forever_internal (hc sw α) s ->
-    (exists a k, reachable (hc sw α) s (hc_r a k) /\ forever_internal α a) \/
-    forever_switching sw α s.
+  (** In addition, we will use the following properties relating
+    reachability in various flavors of the transition system. *)
+
+  Lemma reachable_obs_res_inv {G A} sw (α : rts G A) a a' :
+    reachable (res sw (obs α)) a a' ->
+    reachable (res sw α) a a'.
   Proof.
-    intros Hα Hs1.
-    destruct (classic (forever_switching sw α s)) as [? | Hs2]; auto. left.
-    rewrite forever_internal_nbr in Hs1; eauto using hc_det.
-    rewrite forever_switching_nbr in Hs2; eauto.
-    apply not_and_or in Hs2 as [? | Hs2].
-    {
-      specialize (Hs1 s (reachable_refl _ s)) as (s' & Hs').
-      destruct Hs'. elim H. congruence.
-    }
-    apply not_all_ex_not in Hs2 as [a Hs2].
-    apply not_all_ex_not in Hs2 as [k Hs2].
-    apply not_all_ex_not in Hs2 as [Hak Hs2].
-    exists a, k. split; auto.
-    revert a Hak Hs2. cofix IH. intros.
-    edestruct (Hs1 _ Hak) as (a'' & Ha'').
-    inversion Ha''; clear Ha''; subst.
-    destruct r; try now inversion H2.
-    - simpl in H2. inversion H2; clear H2; subst.
-      econstructor; eauto.
-      eapply IH.
-      + transitivity (hc_r a k); eauto.
-        econstructor; eauto.
-        change (internal _) with (hc_behavior sw (internal a') k).
-        constructor; eauto.
-      + intros (a'' & r & s' & Ha'' & Hr & Hrext & Hs'); eauto 10.
-    - elim Hs2; eauto 10.
+    induction 1 as [a | a1 a2 a3 Ha12 Ha23].
+    - constructor.
+    - clear Ha23.
+      inversion Ha12 as [xa1 r2 Hr2]; clear Ha12; subst.
+      destruct Hr2 as [ | a1' r2 Hr2ext Hr2 Ha1']; [inversion H0 | ].
+      induction Ha1' as [a1 | a1 a1' a1'' Ha1' Ha1''].
+      + eapply reachable_step with a2; eauto.
+        rewrite <- H0. constructor; auto.
+      + eapply reachable_step with a1'; eauto.
+        change (internal a1') with (res_behavior sw (internal a1')).
+        constructor; auto.
   Qed.
 
-  Lemma obs_hc_obs_hc {G A} sw (α : rts G A) s r :
-    deterministic α ->
-    obs (hc sw α) s r ->
-    obs_hc sw α s r.
+  Lemma reachable_res {G A} sw (α : rts G A) a a' :
+    reachable α a a' ->
+    reachable (res sw α) a a'.
   Proof.
-    intros Hα Hr.
-    destruct Hr as [Hs | s' r Hrext Hr Hs'].
-    - apply forever_hc in Hs as [(a & k & Hs' & Ha) | Hs]; auto.
-      + eapply obs_hc_settles.
-        remember (hc_r a k) as s' in Hs'.
-        induction Hs'; eauto using hc_settles_internal.
-        subst. constructor; auto.
-      + eapply obs_hc_forever_switching; eauto.
-    - eapply obs_hc_settles; eauto.
-      induction Hs'; eauto using hc_settles_internal.
-      inversion Hr; clear Hr; subst.
-      destruct r0; simpl in *; (try now inversion Hrext); eauto.
+    induction 1 as [a | a1 a2 a3 Ha2 Ha3]; eauto.
+    eapply reachable_step; eauto.
+    change (internal a2) with (res_behavior sw (internal a2)).
+    constructor; eauto.
   Qed.
 
-  Lemma obs_hc_obs_hc_obs {G A} sw (α : rts G A) s r :
-    obs_hc sw α s r ->
-    obs (hc sw (obs α)) s r.
+  (** Another important key property is is the following: the
+    behaviors of [obs α] will all be external, so that an internal
+    transition in [res sw (obs α)] can only come from internal
+    switching. If there is no such internal switching, and [res sw α]
+    takes an internal step, then it must have come from an internal
+    step of [α]. *)
+
+  Lemma res_noswitch_internal_inv {G A} sw (α : rts G A) a a' :
+    ~ (exists x, res sw (obs α) a (internal x)) ->
+    res sw α a (internal a') ->
+    α a (internal a').
   Proof.
-    intro.
-    destruct H.
-    - induction H.
-      + apply obs_external with (hc_r a k); eauto.
-        subst. constructor.
-        eapply obs_external with a'; eauto.
-        eapply hc_behavior_external; eauto.
-      + apply obs_external with (hc_r a k); eauto.
-        change diverges with (hc_behavior sw diverges k).
-        constructor. auto.
-      + apply obs_reachable with s'; auto.
-        econstructor; eauto.
-        rewrite <- H2. constructor. eauto.
-    - eapply obs_diverges.
-      revert s H. cofix IH. intros.
-      destruct H. econstructor; eauto.
-      rewrite <- H2. constructor. eauto.
+    intros Hnoswitch Ha'.
+    inversion Ha'; clear Ha'; subst.
+    destruct r; try now inversion H.
+    - simpl. auto.
+    - eelim Hnoswitch.
+      exists a'. rewrite <- H. constructor. eauto.
   Qed.
 
-  Lemma obs_hc_obs_hc_obs_sim {G A} sw (α : rts G A) :
+  (** This is used to show the following key property, which spells
+    out the case analysis for the divergence of [res sw α]. *)
+
+  Lemma forever_internal_res_inv {G A} sw (α : rts G A) a :
     deterministic α ->
-    sim eq (obs (hc sw α)) (obs (hc sw (obs α))).
+    forever_internal (res sw α) a ->
+    (exists a', reachable (res sw α) a a' /\ forever_internal α a') \/
+    forever_internal (res sw (obs α)) a.
+  Proof.
+    intros Hα Ha1.
+    destruct (classic (forever_internal (res sw (obs α)) a)) as [? | Ha2]; auto.
+    left.
+    rewrite forever_internal_nbr in Ha1; eauto using res_det.
+    rewrite forever_internal_nbr in Ha2; eauto using res_det, obs_deterministic.
+    apply not_all_ex_not in Ha2 as [a' Ha2].
+    apply not_all_ex_not in Ha2 as [Ha' Ha2].
+    exists a'. split; auto using reachable_obs_res_inv.
+    apply forever_internal_nbr; eauto.
+    intros a'' Ha''.
+    specialize (Ha1 a'') as (a''' & Ha''').
+    - transitivity a'; eauto using reachable_res, reachable_obs_res_inv.
+    - exists a'''.
+      eapply res_noswitch_internal_inv; eauto.
+      intros (a'''' & Ha'''').
+      apply Ha2. exists a''''.
+      inversion Ha''''; clear Ha''''; subst.
+      constructor.
+      eapply obs_reachable; eauto.
+  Qed.
+
+  (** *** External behavior *)
+
+  (** If [res sw α] eventually reaches an externally observable step,
+    this will potentially happen after an interleaving of internal
+    steps of [α], and external steps of [α] that have been turned into
+    internal steps of [res sw α]. We need to decompose those, because
+    on the [obs (res sw (obs α))] side, internal steps of [α] will
+    have been absorbed by the innermost [obs], whereas internal steps
+    introduced by [res] will be absorbed by the outermost [obs].
+
+    This makes the induction on the internal segment in [res sw α]
+    somewhat tricky, because proving that [obs (res sw (obs α))]
+    is invariant under the addition of an additional initial internal
+    step of [res sw α] is complicated. However, the following,
+    equivalent formulation works very well in that context. *)
+
+  Definition obs_res_obs {G A} sw (α : rts G A) r a :=
+    forall x,
+      reachable α x a ->
+      obs (res sw (obs α)) x r.
+
+  Lemma obs_res_obs_internal {G A} sw (α : rts G A) a a' r:
+    res sw α a (internal a') ->
+    obs_res_obs sw α r a' ->
+    obs_res_obs sw α r a.
+  Proof.
+    intros Ha' H x Hx.
+    inversion Ha' as [xa ra Hra]; clear Ha'; subst.
+    destruct ra; try now inversion H1.
+    - (* internal step of α *)
+      inversion H1; clear H1; subst.
+      eapply H; eauto.
+      transitivity a; eauto.
+    - (* external step of α turned internal step of [res α] *)
+      eapply obs_internal; eauto.
+      rewrite <- H1. constructor. eauto.
+  Qed.
+
+  Lemma res_behavior_external {G A} sw (r : behavior G A) :
+    behavior_external (res_behavior sw r) ->
+    behavior_external r.
+  Proof.
+    destruct r; inversion 1; constructor.
+  Qed.
+
+  Lemma obs_res_obs_external {G A} sw (α : rts G A) a a' r :
+    reachable (res sw α) a a' ->
+    res sw (obs α) a' r ->
+    behavior_external r ->
+    obs (res sw (obs α)) a r.
+  Proof.
+    intros Ha' Hr Hrext.
+    cut (obs_res_obs sw α r a).
+    - unfold obs_res_obs. eauto.
+    - induction Ha'; eauto using obs_res_obs_internal.
+      intros x Hx.
+      eapply obs_external with x; eauto.
+      inversion Hr; clear Hr; subst. constructor.
+      eauto using obs_reachable, res_behavior_external.
+  Qed.
+
+  (** *** Main proof *)
+
+  (** Putting these pieces together, *)
+
+  Lemma obs_res_comm {G A} sw (α : rts G A) :
+    deterministic α ->
+    sim eq (obs (res sw α)) (obs (res sw (obs α))).
   Proof.
     intros Hα s _ [] r Hr.
     exists r. split; [ | rauto].
-    apply obs_hc_obs_hc_obs.
-    apply obs_hc_obs_hc; auto.
+    destruct Hr.
+    - edestruct @forever_internal_res_inv as [(s' & Hs' & Hd) | ]; eauto.
+      eapply obs_res_obs_external; eauto.
+      change diverges with (@res_behavior G A sw diverges). constructor.
+      eauto.
+    - apply obs_res_obs_external with a'; auto.
+      inversion H0; clear H0; subst. constructor.
+      eauto using res_behavior_external.
   Qed.
+End Res.
 
+
+(** * Horizontal composition *)
+
+Module HComp.
+  Definition of {li} (α β : modsem (li -o li)) :=
+    Res.of (FComp.of α β).
 End HComp.
